test_databases/include_cycle/literal_child.mm
@@ -1,0 +1,1 @@
+$[ test_databases/include_cycle/literal_root.mm $]
